backends/lean/Aeneas/Tactic/Step/StepArraySpec.lean
@@ -120,7 +120,8 @@ def parseStepArraySpec
     -- Elaborate the full theorem
     elabCommand
       (← `(command| $vis:declModifiers theorem $thm_name:ident $i (_ : Aeneas.Std.UScalar.val $i < Aeneas.Std.Array.length $array) :
-            Aeneas.Std.WP.spec (Aeneas.Std.Array.index_usize $array $i) (fun $x:ident => $pred) :=
+            Aeneas.Std.WP.spec (Aeneas.Std.Array.index_usize $array $i)
+              (Aeneas.Std.WP.successPost (fun $x:ident => $pred)) :=
             Aeneas.Std.Array.index_usize_const_spec (fun $i:ident $x:ident => $pred) (fun $i:ident $x:ident => $pred)
             $array (by simp) (by $tac) $i (by scalar_tac) (by scalar_tac)))
   | _ => throwUnsupportedSyntax
